.

src/program_proof/session/session_definitions.v
@@ -142,13 +142,13 @@ Module Operation.
   Context {u64_hsEq: SessionPrelude.hsEq u64 (well_formed := u64_well_formed)}.
 
   #[global]
-  Instance hsEq_Operation (n: nat) : SessionPrelude.hsEq (Operation.t u64) (well_formed := well_formed n) :=
+  Instance hsEq (n: nat) : SessionPrelude.hsEq (Operation.t u64) (well_formed := well_formed n) :=
     SessionPrelude.hsEq_preimage getVersionVector.
 
   Context {u64_hsOrd: SessionPrelude.hsOrd u64 (well_formed := u64_well_formed)}.
 
   #[global]
-  Instance hsOrd_Operation (n: nat) : SessionPrelude.hsOrd (Operation.t u64) (well_formed := well_formed n) :=
+  Instance hsOrd (n: nat) : SessionPrelude.hsOrd (Operation.t u64) (well_formed := well_formed n) :=
     SessionPrelude.hsOrd_preimage getVersionVector.
 
   End HASKELLISH_INSTANCES.
@@ -885,6 +885,165 @@ Module ClientSide.
   End Coq_nat.
 
 End ClientSide.
+
+Section properties.
+
+Import ServerSide SessionPrelude.
+
+Lemma redefine_coq_lexicographicCompare
+  : coq_lexicographicCompare = vectorGt.
+Proof.
+  reflexivity.
+Defined.
+
+Lemma redefine_coq_equalSlices
+  : coq_equalSlices = vectorEq.
+Proof.
+  reflexivity.
+Defined.
+
+Lemma redefine_coq_sortedInsert (n: nat)
+  : coq_sortedInsert = sortedInsert (hsOrd := Operation.hsOrd n).
+Proof.
+  reflexivity.
+Defined.
+
+#[local] Hint Resolve @Forall_True : core.
+
+Lemma aux0_equalSlices l1 l2 :
+  length l1 = length l2 ->
+  coq_equalSlices l1 l2 = true ->
+  l1 = l2.
+Proof.
+  rewrite redefine_coq_equalSlices. intros. rewrite <- vectorEq_true_iff; eauto 2.
+Qed.
+
+Lemma aux1_equalSlices l1 l2 :
+  length l1 = length l2 ->
+  coq_equalSlices l1 l2 = false ->
+  l1 ≠ l2.
+Proof.
+  rewrite redefine_coq_equalSlices. intros. rewrite <- vectorEq_true_iff; eauto 2.
+  rewrite H0; congruence.
+Qed.
+
+Lemma aux2_equalSlices l1 l2 b :
+  length l1 = length l2 ->
+  coq_equalSlices l1 l2 = b ->
+  coq_equalSlices l2 l1 = b.
+Proof.
+  rewrite redefine_coq_equalSlices. intros. subst b. eapply (eqb_comm (hsEq_A := hsEq_vector (length l1))); eauto.
+Qed.
+
+Lemma aux3_equalSlices l :
+  coq_equalSlices l l = true.
+Proof.
+  change (coq_equalSlices l l) with (eqb (hsEq := hsEq_vector (length l)) l l).
+  rewrite eqb_eq; eauto 2. eapply eqProp_reflexivity; eauto 2.
+Qed.
+
+Lemma aux0_lexicographicCompare l1 l2 l3 :
+  coq_lexicographicCompare l2 l1 = true ->
+  coq_lexicographicCompare l3 l2 = true ->
+  coq_lexicographicCompare l3 l1 = true.
+Proof.
+  rewrite redefine_coq_lexicographicCompare.
+  intros. eapply vectorGt_transitive; eauto.
+Qed.
+
+Lemma aux1_lexicographicCompare l1 l2 :
+  length l1 = length l2 -> 
+  l1 ≠ l2 ->
+  (coq_lexicographicCompare l2 l1 = false <-> coq_lexicographicCompare l1 l2 = true).
+Proof.
+  rewrite redefine_coq_lexicographicCompare. remember (length l1) as len eqn: len_eq.
+  pose proof (ltProp_trichotomy (hsOrd := hsOrd_vector len) l1 l2) as claim. simpl in claim.
+  symmetry in len_eq. intros len_eq'. symmetry in len_eq'.
+  specialize (claim (conj (Forall_True _) len_eq) (conj (Forall_True _) len_eq')).
+  destruct claim as [H_lt | [H_eq | H_gt]].
+  - rewrite H_lt. intros NE. split.
+    { congruence. }
+    intros l1_gt_l2. contradiction (ltProp_irreflexivity (hsOrd := hsOrd_vector len) l1 l1); eauto.
+    + eapply eqProp_reflexivity; eauto.
+    + eapply ltProp_transitivity with (y := l2); eauto.
+  - intros NE. contradiction NE. clear NE. rewrite <- vectorEq_true_iff; eauto 2.
+    change (eqb (hsEq := hsEq_vector len) l1 l2 = true). rewrite eqb_eq; eauto 2.
+  - rewrite H_gt. intros NE. split.
+    { congruence. }
+    intros _. change (ltb (hsOrd := hsOrd_vector len) l1 l2 = false).
+    rewrite ltb_nlt; eauto 2. intros NLT. change (ltb (hsOrd := hsOrd_vector len) l2 l1 = true) in H_gt.
+    rewrite ltb_lt in H_gt; eauto 2. contradiction (ltProp_irreflexivity (hsOrd := hsOrd_vector len) l1 l1); eauto.
+    + eapply eqProp_reflexivity; eauto.
+    + eapply ltProp_transitivity with (y := l2); eauto.
+Qed.
+
+Lemma aux3_lexicographicCompare l1 l2 :
+  length l1 = length l2 ->
+  coq_lexicographicCompare l2 l1 = false ->
+  coq_lexicographicCompare l1 l2 = false ->
+  l1 = l2.
+Proof.
+  rewrite redefine_coq_lexicographicCompare. intros. rewrite <- vectorEq_true_iff; eauto 2.
+  change (eqb (hsEq := hsEq_vector (length l1)) l1 l2 = true). rewrite eqb_eq; eauto 2.
+  pose proof (ltProp_trichotomy (hsOrd := hsOrd_vector (length l1)) l1 l2) as [H_lt | [H_eq | H_gt]]; eauto.
+  - rewrite <- ltb_lt in H_lt; eauto 2. simpl in *. congruence.
+  - rewrite <- ltb_lt in H_gt; eauto 2. simpl in *. congruence.
+Qed.
+
+Lemma aux4_lexicographicCompare l1 l2 :
+  coq_lexicographicCompare l1 l2 = true ->
+  coq_equalSlices l1 l2 = false.
+Proof.
+  rewrite redefine_coq_lexicographicCompare. rewrite redefine_coq_equalSlices.
+  intros. eapply vectorGt_implies_not_vectorEq; eauto 2.
+Qed.
+
+Lemma aux5_lexicographicCompare l1 l2 :
+  coq_equalSlices l1 l2 = true ->
+  coq_lexicographicCompare l1 l2 = false.
+Proof.
+  rewrite redefine_coq_lexicographicCompare. rewrite redefine_coq_equalSlices.
+  intros. eapply vectorEq_implies_not_vectorGt; eauto 2.
+Qed.
+
+Lemma aux6_lexicographicCompare l1 l2 :
+  length l1 = length l2 ->
+  coq_lexicographicCompare l1 l2 = false ->
+  (coq_lexicographicCompare l2 l1 = true \/ l1 = l2).
+Proof.
+  rewrite redefine_coq_lexicographicCompare. intros.
+  pose proof (ltProp_trichotomy (hsOrd := hsOrd_vector (length l2)) l1 l2) as [H_lt | [H_eq | H_gt]]; eauto.
+  - rewrite <- eqb_eq in H_eq; eauto 2. simpl in *. right; eapply aux0_equalSlices; trivial.
+  - rewrite <- ltb_lt in H_gt; eauto 2. simpl in *. congruence.
+Qed.
+
+Definition is_sorted (l: list (Operation.t nat)) : Prop :=
+  ∀ i, ∀ j, (i < j)%nat -> ∀ o1, ∀ o2, l !! i = Some o1 -> l !! j = Some o2 ->
+  coq_lexicographicCompare o2.(Operation.VersionVector) o1.(Operation.VersionVector) = true.
+
+Lemma redefine_is_sorted n l
+  : is_sorted l = isSorted (hsOrd := Operation.hsOrd n) l.
+Proof.
+  reflexivity.
+Defined.
+
+Lemma coq_maxTS_length n xs ys
+  (LEN1: length xs = n)
+  (LEN2: length ys = n)
+  : length (coq_maxTS xs ys) = n.
+Proof.
+  revert xs ys LEN1 LEN2; induction n as [ | n IH], xs as [ | x xs], ys as [ | y ys]; simpl in *; intros; try congruence; f_equal; eapply IH; word.
+Qed.
+
+Lemma coq_sortedInsert_length l i
+  : (length (coq_sortedInsert l i) <= length l + 1)%nat.
+Proof.
+  induction l as [ | x l IH]; simpl; try word.
+  destruct (coq_lexicographicCompare _ _) as [ | ]; simpl; try word.
+  destruct (coq_equalSlices _ _) as [ | ]; simpl; try word.
+Qed.
+
+End properties.
 
 Section heap.
 
